processes/beta.v
@@ -1,0 +1,229 @@
+From DST Require Import sort.unscoped sort.sort sort.beta sort.sortcheck processes.process.
+From Paco Require Import paco.
+Require Import String List ZArith Relations.
+Local Open Scope string_scope.
+Import ListNotations.
+Require Import Setoid Morphisms.
+
+Inductive mqueue: Type := 
+  | nilq: mqueue
+  | mesq: participant -> label -> sort -> mqueue -> mqueue.
+
+Fixpoint conq (m1 m2: mqueue): mqueue :=
+  match m1 with
+    | nilq         => m2
+    | mesq p l v q => mesq p l v (conq q m2)
+  end.
+
+Inductive session: Type :=
+  | sind: participant -> process -> mqueue -> session
+  | spar: session -> session -> session.
+
+Notation "p '<--' P '|' h" :=  (sind p P h) (at level 50, no associativity).
+Notation "s1 '|||' s2" :=  (spar s1 s2) (at level 50, no associativity): type_scope.
+
+Inductive qcong: relation mqueue :=
+  | qcons : forall {A B: Type} q1 q2 l1 l2 v1 v2 h1 h2, q1 <> q2 -> 
+                                             qcong (conq h1 (conq (mesq q1 l1 v1 nilq) (conq (mesq q2 l2 v2 nilq) h2)))
+                                                   (conq h1 (conq (mesq q2 l2 v2 nilq) (conq (mesq q1 l1 v1 nilq) h2)))
+  | qnilL : forall h, qcong (conq nilq h) h
+  | qnilR : forall h, qcong h (conq nilq h)
+  | qassoc: forall h1 h2 h3, qcong (conq h1 (conq h2 h3)) (conq (conq h1 h2) h3).
+
+Definition subst_expr (p: process) (l: label) (e: sort): process :=
+  match p with
+    | ps_receive s0 s1  => 
+      let fix next lst :=
+      match lst with
+        | (pair (pair lbl (svar 0)) P)::xs => 
+          if eqb lbl l then
+          let fix rec P :=
+            match P with
+              | ps_send pt l e1 P => ps_send pt l (subst_sort (e .: svar) e1) (rec P)
+              | ps_ite e1 P Q     => ps_ite (subst_sort (e .: svar) e1) (rec P) (rec Q)
+              | ps_receive s2 s3  => ps_receive s2 ((list_map (prod_map (prod_map (fun x => x) (fun x => x)) (rec))) s3)
+              | ps_mu P           => ps_mu (rec P)
+              | _                 => P
+            end
+          in rec P
+          else next xs
+       | (pair (pair lbl _) P)::xs => next xs
+       | _                         => p
+     end
+     in next s1
+    | _                            => p
+  end.
+
+(* Definition PBob'': process :=
+  ps_receive "Alice" (cons (pair (pair "l1" (svar 0)) (ps_send "Carol" "l2" (svar 0) (ps_send "Burak" "l3" (svar 100) (ps_send "Cagin" "l4" (svar 88) ps_end))))
+                     (cons (pair (pair "l4" (svar 0)) (ps_send "Carol" "l2" (slambda (svar 0) sint (slambda (svar 0) sint (splus (splus (svar 1) (svar 0)) (svar 2))))
+                       (ps_receive "Alice" 
+                         (cons (pair (pair "l4" (svar 0)) (ps_send "Marol" "l3" (slambda (svar 0) sint (sminus (svar 0) (svar 2))) (ps_send "Burak" "l2" (svar 0) (ps_send "Cagin" "l4" (svar 1) ps_end))))
+                         (cons (pair (pair "l1" (svar 0)) (ps_send "Zarol" "l2" (svar 0) ps_end)) nil))))) nil)
+                     ).
+
+Eval compute in (subst_expr PBob'' "l4" (sci 43)).
+
+Definition pp := (ps_receive "Alice"
+            (cons
+               (pair (pair "l4" (svar 0))
+                  (ps_send "Marol" "l3" (slambda (svar 0) sint (sminus (sci 43) (svar 1))) (ps_send "Burak" "l2" (sci 43) (ps_send "Cagin" "l4" (svar 0) ps_end))))
+               (cons (pair (pair "l1" (svar 0)) (ps_send "Zarol" "l2" (sci 43) ps_end)) nil))).
+
+Eval compute in (subst_expr pp "l4" (sci 88)). *)
+
+
+(* Inductive pcong: relation process :=
+  | pmuUnf: forall {A: Type} p v, pcong (ps_mu p) (@unfold_mu A v p). *)
+
+Inductive scong: relation session :=
+  | sann   : forall p M, scong ((p <-- ps_end | nilq) ||| M) M
+  | scomm  : forall M1 M2, scong (M1 ||| M2) (M2 ||| M1)
+  | sassoc : forall M1 M2 M3, scong (M1 ||| M2 ||| M3) (M1 ||| (M2 ||| M3))
+(*| sassoc2: forall M1 M2 M3, scong (M1 ||| M2 ||| M3) ((M1 ||| M2) ||| M3) *)
+  | sassoc2: forall M1 M2 M3, scong (M1 ||| M2 ||| M3) (M1 ||| (M3 ||| M2)).
+ (* | scongl : forall p P Q h1 h2 M, pcong P Q -> qcong h1 h2 -> 
+                                   scong ((p <-- P | h1) ||| M) ((p <-- Q | h2) ||| M). *)
+Inductive beta: relation session :=
+  | r_send : forall p q l e P hp M, 
+                                beta ((p <-- (ps_send q l e P) | hp) ||| M) 
+                                     ((p <-- P | conq hp (mesq q l e nilq)) ||| M)
+  | r_rcv   : forall p q l xs v Q hp hq M,
+                                beta ((p <-- ps_receive q xs | hp) ||| (q <-- Q | conq (mesq p l v nilq) hq) ||| M)
+                                     ((p <-- subst_expr (ps_receive q xs) l v | hp)  ||| (q <-- Q | hq) ||| M)
+  | r_cond_t: forall p P Q h M, beta ((p <-- ps_ite (scb true) P Q | h) ||| M) ((p <-- P | h) ||| M)
+  | r_cond_f: forall p P Q h M, beta ((p <-- ps_ite (scb false) P Q | h) ||| M) ((p <-- Q | h) ||| M).
+(*   | r_struct: forall M1 M1' M2 M2', scong M1 M1' -> scong M2' M2 -> beta M1' M2' -> beta M1 M2. *)
+
+Declare Instance Equivalence_beta : Equivalence beta.
+Declare Instance Equivalence_scong : Equivalence scong.
+
+Inductive multi {X : Type} (R : relation X) : relation X :=
+  | multi_refl : forall (x : X), multi R x x
+  | multi_step : forall (x y z : X), R x y -> multi R y z -> multi R x z.
+
+Definition beta_multistep := multi beta.
+
+#[global]
+Declare Instance RW_scong3: Proper (scong ==> scong ==> impl) beta.
+#[global]
+Declare Instance RW_scong4: Proper (scong ==> scong ==> impl) beta_multistep.
+
+Local Open Scope string_scope.
+
+Definition M1 (p q: participant) (l: label) : session :=
+  (p <-- ps_receive q (cons (pair (pair l (svar 0)) ps_end) nil) | nilq) ||| (q <-- ps_send p l (sci 42) ps_end | nilq).
+
+Definition M1' (p q: participant) (l: label): session :=
+  (p <-- ps_end | nilq) ||| (q <-- ps_end | nilq).
+
+Example redM1: forall (p q: participant) (l: label), beta_multistep (M1 p q l) (M1' p q l).
+Proof. intros.
+       unfold beta_multistep, M1, M1'.
+       setoid_rewrite scomm.
+       apply multi_step with (y := 
+         ((q <-- ps_end | (conq nilq (mesq p l (sci 42) nilq))) ||| 
+          (p <-- ps_receive q (cons (pair (pair l (svar 0)) ps_end) nil) | nilq))).
+       apply r_send. simpl.
+       setoid_rewrite scomm.
+       apply multi_step with (y := 
+         (((p <-- subst_expr (ps_receive q (cons (pair (pair l (svar 0)) ps_end) nil)) l (sci 42) | nilq) ||| 
+          (q <-- ps_end | nilq)))).
+       specialize (r_rcv p q l (cons (pair (pair l (svar 0)) ps_end) nil)
+                         (sci 42) (ps_end) nilq nilq
+                         (p <-- ps_end | nilq)
+       ); intro HR.
+       setoid_rewrite scomm in HR.
+       setoid_rewrite sann in HR.
+       exact HR.
+
+       simpl.
+       rewrite String.eqb_refl.
+       apply multi_refl.
+Qed.
+
+(* Example 2 in "A Very Gentle Introduction to Multiparty Session Types" *)
+Definition PAlice: process := 
+  ps_send "Bob" "l1" (sci 50) (ps_receive "Carol" (cons (pair (pair "l3" (svar 0)) ps_end) nil)).
+
+Definition PBob: process :=
+  ps_receive "Alice" (cons (pair (pair "l1" (svar 0)) (ps_send "Carol" "l2" (sci 100) ps_end))
+                     (cons (pair (pair "l4" (svar 0)) (ps_send "Carol" "l2" (sci 2) ps_end)) nil)).
+
+Definition PCarol: process :=
+  ps_receive "Bob" (cons (pair (pair "l2" (svar 0)) (ps_send "Alice" "l3" (splus (svar 0) (sci 1)) ps_end)) nil).
+
+Definition MS: session := ("Alice" <-- PAlice | nilq) ||| ("Bob" <-- PBob | nilq) ||| ("Carol" <-- PCarol | nilq).
+
+Definition MS': session := ("Alice" <-- ps_end | nilq) ||| ("Bob" <-- ps_end | nilq) ||| ("Carol" <-- ps_end | nilq).
+
+Example redMS: beta_multistep MS MS'.
+Proof. unfold beta_multistep, MS, MS', PAlice.
+       apply multi_step with
+       (y := (("Alice" <-- (ps_receive "Carol" (cons (pair (pair "l3" (svar 0)) ps_end) nil)) | conq nilq (mesq "Bob" "l1" (sci 50) nilq)) ||| 
+             ("Bob" <-- PBob | nilq)) ||| ("Carol" <-- PCarol | nilq)).
+       setoid_rewrite sassoc.
+       apply r_send. simpl.
+
+       setoid_rewrite sassoc.
+       setoid_rewrite scomm.
+       setoid_rewrite sassoc2.
+       setoid_rewrite <- sassoc.
+
+       unfold PBob at 1.
+
+       apply multi_step with
+       (y := ("Bob" <-- subst_expr (PBob) "l1" (sci 50) | nilq)
+              ||| ("Alice" <-- (ps_receive "Carol" (cons (pair (pair "l3" (svar 0)) ps_end) nil)) | nilq)
+              ||| ("Carol" <-- PCarol | nilq)).
+       apply r_rcv.
+       unfold PBob at 1.
+       simpl.
+(*        unfold PCarol. *)
+
+       setoid_rewrite sassoc2.
+       setoid_rewrite <- sassoc.
+
+       apply multi_step with
+       (y := ((("Bob" <-- ps_end | conq nilq (mesq "Carol" "l2" (sci 100) nilq) )
+               ||| ("Carol" <-- (ps_receive "Bob" (cons (pair (pair "l2" (svar 0)) (ps_send "Alice" "l3" (splus (svar 0) (sci 1)) ps_end)) nil)) | nilq))
+               ||| ("Alice" <-- (ps_receive "Carol" (cons (pair (pair "l3" (svar 0)) ps_end) nil)) | nilq))).
+       setoid_rewrite sassoc.
+       apply r_send. simpl.
+
+       setoid_rewrite sassoc.
+       setoid_rewrite scomm.
+       setoid_rewrite sassoc2.
+       setoid_rewrite <- sassoc.
+
+       apply multi_step with
+       (y := ((("Carol" <-- subst_expr (ps_receive "Bob" (cons (pair (pair "l2" (svar 0)) (ps_send "Alice" "l3" (splus (svar 0) (sci 1)) ps_end)) nil)) "l2" (sci 100) | nilq)
+                 ||| ("Bob" <-- ps_end | nilq))
+                 ||| ("Alice" <-- (ps_receive "Carol" (cons (pair (pair "l3" (svar 0)) ps_end) nil)) | nilq))).
+       apply r_rcv. simpl.
+
+       setoid_rewrite sassoc2.
+       setoid_rewrite <- sassoc.
+
+       apply multi_step with
+       (y := ((("Carol" <-- ps_end | conq nilq (mesq "Alice" "l3" (splus (sci 100) (sci 1)) nilq) )
+               ||| ("Alice" <-- (ps_receive "Carol" (cons (pair (pair "l3" (svar 0)) ps_end) nil)) | nilq))
+               ||| ("Bob" <-- ps_end | nilq))).
+       setoid_rewrite sassoc. simpl.
+       apply r_send. simpl.
+
+       setoid_rewrite sassoc.
+       setoid_rewrite scomm.
+       setoid_rewrite sassoc2.
+       setoid_rewrite <- sassoc.
+
+      apply multi_step with
+      (y := ((("Alice" <-- subst_expr (ps_receive "Carol" (cons (pair (pair "l3" (svar 0)) ps_end) nil))
+                                      "l3" (splus (sci 100) (sci 1)) | nilq) 
+             ||| ("Carol" <-- ps_end | nilq))
+             ||| ("Bob" <-- ps_end | nilq))).
+      apply r_rcv. simpl.
+
+      apply multi_refl.
+Qed.
+
